code/ecdsa/Hacl.Impl.EC.Setup.fst
@@ -572,4 +572,21 @@ let uploadA #c a =
       assert_norm(18446744073709551612 + 17179869183 * pow2 64 + 18446744056529682436 * pow2 64 * pow2 64 * pow2 64 = (aCoordinate #P256 % prime256) * pow2 256 % prime256)
 
     |P384 -> 
-      admit()
+            upd a (size 0) (u64 18446744073709551612);
+      upd a (size 1) (u64 17179869183);
+      upd a (size 2) (u64 0);
+      upd a (size 3) (u64 18446744056529682436);
+      
+      let prime = getPrime c in 
+      lemmaToDomain #c #DH (aCoordinate #c % prime);
+      assert_norm(18446744073709551612 + 17179869183 * pow2 64 + 18446744056529682436 * pow2 64 * pow2 64 * pow2 64 = (aCoordinate #P256 % prime256) * pow2 256 % prime256)
+    |Default ->
+      upd a (size 0) (u64 18446744073709551612);
+      upd a (size 1) (u64 17179869183);
+      upd a (size 2) (u64 0);
+      upd a (size 3) (u64 18446744056529682436);
+      
+      let prime = getPrime c in 
+      lemmaToDomain #c #DH (aCoordinate #c % prime);
+      assert_norm(18446744073709551612 + 17179869183 * pow2 64 + 18446744056529682436 * pow2 64 * pow2 64 * pow2 64 = (aCoordinate #P256 % prime256) * pow2 256 % prime256)
+
