specs/ecdsap256/Spec.ECC.Radix.fst
@@ -1,0 +1,79 @@
+module Spec.ECC.Radix
+
+open FStar.Mul
+
+open Lib.ByteSequence
+open Lib.IntTypes
+open Lib.Sequence
+open Lib.RawIntTypes
+
+open Lib.LoopCombinators 
+
+open FStar.Math.Lemmas
+open FStar.Math.Lib
+
+open Spec.ECC.Curves
+
+open Spec.ECC
+
+
+let radix = 4
+
+val getPrecomputedPoint: #c: curve -> p: point_nat_prime #c -> i: nat -> 
+  Tot (r: point_nat_prime #c {pointEqual r (point_mult i p)})
+
+let getPrecomputedPoint #c p i = 
+  point_mult i p
+
+
+val _ml_step: #c: curve -> k: scalar_bytes #c 
+  -> p0: point_nat_prime #c  
+  -> i: nat{i < v (getScalarLen c)} 
+  -> p: point_nat_prime #c
+  -> point_nat_prime #c
+
+let _ml_step #c k p0 i p =
+  let s = scalar_as_nat k in 
+  let si = (arithmetic_shift_right s (i * radix)) % (pow2 radix) in 
+  let pointPrecomputed = getPrecomputedPoint p0 si in 
+
+  (* lazy version *)
+  let p2 = _point_double p in 
+  let p4 = _point_double p2 in 
+  let p8 = _point_double p4 in 
+  let p16 = _point_double p8 in
+  
+  _point_add pointPrecomputed p16
+
+
+
+assume val pred0: #c: curve -> x: point_nat_prime #c -> s: scalar_bytes #c ->
+  p: point_nat_prime #c -> i: nat {i < v (getScalarLen c)} ->
+  Lemma (True)
+
+val lemma_predicate0:  #c: curve -> s: scalar_bytes #c -> p: point_nat_prime #c -> 
+  Lemma (True)
+
+let lemma_predicate0 #c s p = 
+  let pred = pred0 #c in
+  Classical.forall_intro_4 pred
+
+
+val radix_spec: #c: curve -> s: scalar_bytes #c 
+  -> i: point_nat_prime #c
+  -> r: point_nat_prime #c {
+    (* r == repeati (v (getScalarLen c)) (_ml_step #c s) i /\ *)
+    pointEqual r (point_mult (scalar_as_nat #c s) i)}
+
+
+let radix_spec #c s i = 
+  let len : nat  = v (getScalarLen c) in 
+  
+  let pred i r = True in
+    
+  let f = _ml_step #c s i in 
+
+  lemma_predicate0 s i;
+  admit();
+  repeati_inductive' #(point_nat_prime #c) len pred f i
+
